MirrorCharge!/src/MirrorCharge/Java/Semantics.v
@@ -1,9 +1,11 @@
 Require Import Charge.Logics.ILogic.
+Require Import Charge.Logics.Later.
 Require Import Charge.Logics.ILEmbed.
 Require Import Charge.Open.OpenILogic.
 Require Import Charge.Open.Subst.
 
 Require Import Java.Language.Lang.
+Require Import Java.Language.Program.
 
 Require Import Java.Semantics.OperationalSemantics.
 Require Import Java.Semantics.AxiomaticSemantics.
@@ -38,57 +40,120 @@ Proof.
   intros.
   eapply roc_post; [eapply rule_skip | apply H].
 Qed.
-
+	
 Lemma rule_if (e : dexpr) c1 c2 (P Q : sasn) G
       (Hc1 : G |-- {[(@embed (@vlogic String.string _) sasn _ 
-      				  (ap (T := Fun stack)
-      				      (ap (pure (@eq sval)) (eval2 e)) 
-      				  (pure (vbool true)))) //\\ P]} c1 {[Q]})
+                      ap_eq [eval2 e, pure (vbool true)]) //\\ P]} c1 {[Q]})
       (Hc2 : G |-- {[(@embed (@vlogic String.string _) sasn _ 
-      				  (ap (T := Fun stack)
-      				      (ap (pure (@eq sval)) (eval2 (E_not e))) 
-      				  (pure (vbool true)))) //\\ P]} c2 {[Q]}) :
+                      ap_eq [eval2 (E_not e), pure (vbool true)]) //\\ P]} c2 {[Q]}) :
   G |-- {[P]} cif e c1 c2 {[Q]}.
 Proof.
   eapply rule_if; unfold vlogic_eval, Open.liftn, Open.lift; simpl in *;
   	[apply Hc1|apply Hc2].
 Qed.
 
-Check subst2.
   Lemma rule_read_fwd (x y : String.string) (f : String.string) (e : stack -> sval) (P : sasn) (G : spec)
     (HPT : P |-- ap (T := Fun stack) (ap (ap (pure pointsto2) (stack_get y)) (pure f)) e) : 
     G |-- {[ P ]} 
-              cread x y f 
-              {[ Exists v : sval, (*(@embed (@vlogic String.string _) sasn _)
-    								      (ap (T := Fun stack) 
-    								          (ap (pure (@eq sval)) (stack_get x)) 
-    								          (apply_subst2 sval e (subst2 (pure v) x)))  //\\ *)
-    							   (apply_subst2 asn P (subst2 (pure (T := Fun stack) v) x)) ]}.
+          cread x y f 
+          {[ Exists v : sval, embed (ap_eq [stack_get x, apply_subst2 sval e (subst2 (pure v) x)]) //\\ 
+    					      (apply_subst2 asn P (subst2 (pure (T := Fun stack) v) x)) ]}.
   Proof.
-admit.
-(*
-    pose proof @rule_read_fwd x y f e P. unfold Open.liftn, Open.lift, open_eq, stack_get, Open.var_expr in *; simpl in *.
+    pose proof @rule_read_fwd x y f e P. 
+    unfold Open.liftn, Open.lift, open_eq, stack_get, Open.var_expr in *; simpl in *.
 	rewrite <- H; [apply ltrueR | apply HPT].
-*)
   Qed.
 
 Require Import Charge.Logics.BILogic.
 
   Lemma rule_write_fwd (x f : String.string) (e : dexpr) G (P Q : sasn) (e' : stack -> sval)
-        (HPT : P |-- Q ** ap (T := Fun stack) (ap (ap (pure pointsto2) (stack_get x)) (pure f)) e') :
-    G |-- ({[ P ]} cwrite x f e {[ Q ** ap (T := Fun stack) (ap (ap (pure pointsto2) (stack_get x)) (pure f)) (eval2 e)]}).
+        (HPT : P |-- Q ** ap_pointsto [x, f, e']) :
+    G |-- ({[ P ]} cwrite x f e {[ Q ** ap_pointsto [x, f, eval2 e]]}).
   Proof.
      pose proof @rule_write_frame G P Q x f e' e. unfold Open.liftn, Open.lift, open_eq, stack_get, Open.var_expr in *; simpl in *.
 	 apply H; apply HPT.
   Qed.
 
   Lemma rule_assign_fwd x (e : dexpr) G P :
-    G |-- {[ P ]} cassign x e {[ Exists v : sval, (@embed (@vlogic String.string _) sasn _)
-    								      (ap (T := Fun stack) 
-    								          (ap (pure (@eq sval)) (stack_get x)) 
-    								          (apply_subst2 sval (eval2 e) (subst2 (pure v) x))) //\\ 
+    G |-- {[ P ]} cassign x e {[ Exists v : sval,
+                                 embed (ap_eq [stack_get x, 
+                                               apply_subst2 sval (eval2 e) (subst2 (pure v) x)]) //\\ 
     							   (apply_subst2 asn P (subst2 (pure (T := Fun stack) v) x)) ]}.
   Proof.
     pose proof @rule_assign_fwd G P.
     apply H. reflexivity.
   Qed.
+
+Definition set_fold_fun (x f : String.string) (P : sasn) :=
+	ap_pointsto [x, f, pure null] ** P.
+
+  Lemma rule_alloc_fwd (x C : String.string) (G : spec) (P : sasn) (fields : SS.t) (Pr : Prog_wf) 
+	(Heq : G |-- prog_eq Pr)
+	(Hf : field_lookup2 Pr C fields) :
+	G |-- {[ P ]} calloc x C {[ Exists p : ptr, embed (ap_typeof [x, C] //\\
+	                                            ap_eq [stack_get x, pure (vptr p)]) //\\
+	                                            SS.fold (set_fold_fun x) fields 
+	                                                    (apply_subst2 asn P (subst2 (pure (T := Fun stack) p) x)) ]}.
+  Proof.
+  	admit.
+  Qed.
+
+Require Import List.
+
+  Lemma rule_static_complete C (m : String.string) (ps : list String.string) (es : list dexpr) (x r : var) G
+    (P Q F Pm Qm : sasn)
+    (HSpec : G |-- |> method_spec2 C m ps r Pm Qm)
+    (HPre: P |-- apply_subst2 asn Pm (substl_trunc (zip ps (@map _ (stack -> sval) eval2 es))) ** F)
+    (HLen: length ps = length es)
+    (HPost : Exists v:sval, apply_subst2 asn Qm (substl_trunc (zip (@cons String.string r ps) 
+                                     (@cons (stack -> sval) (stack_get x)
+                                      (@map (stack -> sval) _ (fun e => apply_subst2 sval e (subst2 (pure (T := Fun stack) v) x)) 
+                                          (@map dexpr (stack -> sval) eval2 es))))) ** 
+                           apply_subst2 asn F (subst2 (pure (T := Fun stack) v) x) |-- Q) :
+          G |-- {[ P ]} cscall x C m es {[ Q ]}.
+Proof.
+
+    
+(*
+    reify_imp (G |-- |> method_spec2 C m ps r Pm Qm).
+    reify_imp (P |-- apply_subst2 asn Pm (substl_trunc (zip ps (@map _ (stack -> sval) eval2 es))) ** F).
+    reify_imp (apply_subst2 asn Pm (substl_trunc (@nil ((String.string * (stack -> sval)%type))))).
+*)
+	reify_imp (Exists x : asn, (pure (T := Fun stack) x)).
+	reify_imp (fun x : sval => ap_eq [pure (T := Fun stack) x, pure (T := Fun stack) x]).
+	reify_imp (Exists x : sval, ap_eq [(pure (T := Fun stack) x), pure (T := Fun stack) (vint 2)]).
+
+reify_imp (Exists v:sval, apply_subst2 asn Qm (substl_trunc (zip (@cons String.string r ps) 
+                                     (@cons (stack -> sval) (stack_get x)
+                                      (@map (stack -> sval) _ (fun e => apply_subst2 sval e (subst2 (pure (T := Fun stack) v) x)) 
+                                          (@map dexpr (stack -> sval) eval2 es))))) ** 
+                           apply_subst2 asn F (subst2 (pure (T := Fun stack) v) x) |-- Q).
+                           (reify_imp (fun (x y : nat) => x)).
+                           
+    reify_imp (exists x : nat, x = x).                     
+	reify_imp (Exists x : nat, ap_eq [(pure (T := Fun stack) x), pure (T := Fun stack) (vint 2)]).
+    reify_imp (@map (stack -> sval) _ (fun e => apply_subst2 sval e (subst2 (pure (T := Fun stack) (vint 0)) x))
+    	 		(@map _ (stack -> sval) eval2 es)).
+    reify_imp (@cons String.string r ps).
+    reify_imp (@zip String.string (stack -> sval) (@cons String.string r ps) 
+    	(@cons (stack -> sval) (stack_get x)
+        (@map (stack -> sval) _ (fun e => apply_subst2 sval e (subst2 (pure (T := Fun stack) (vint 0)) x)) 
+        (@map dexpr (stack -> sval) eval2 es)))).
+    reify_imp (Exists v:sval, apply_subst2 asn Qm  (substl_trunc (zip (r :: ps) ((stack_get x) ::
+                                      map (fun e => apply_subst2 sval e (subst2 (pure (T := Fun stack) v) x)) 
+                                          (@map dexpr (stack -> sval) eval2 es)))) ** 
+                           apply_subst2 asn F (subst2 (pure (T := Fun stack) v) x) |-- Q).
+    reify_imp (map (fun e => apply_subst2 sval e (subst2 (pure (T := Fun stack) (vint 0)) x)) 
+                                          (@map dexpr (stack -> sval) eval2 es)).
+    reify_imp (map dexpr (stack -> sval) eval2 es).
+
+
+(*
+  
+  
+  Lemma rule_alloc_ax (x : var) C fields :
+    [prog](fun Pr => field_lookup Pr C fields) |-- {[ ltrue ]} calloc x C {[ Exists p:ptr,
+      @lembedand vlogic sasn _ _ (@land vlogic _ (`typeof `C (x/V)) (open_eq x /V `(vptr p)))
+      (SS.fold (fun f Q => `pointsto `(vptr p) `f `null ** Q) fields ltrue)]}.
+  Proof.
+*)
