MirrorCharge!/src/MirrorCharge/Java/Syntax.v
@@ -37,9 +37,15 @@ Local Instance Applicative_Fun A : Applicative (Fun A) :=
 
 Inductive typ :=
 | tyArr : typ -> typ -> typ
+| tyList : typ -> typ
+| tyPair : typ -> typ -> typ
+
+(*
 | tyVarList : typ
 | tyExprList : typ
 | tySubstList : typ
+*)
+
 | tyVal : typ
 | tyString : typ
 | tyNat : typ
@@ -55,6 +61,10 @@ Inductive typ :=
 
 Notation "'tyPure'" := (tyArr tyStack tyProp).
 Notation "'tySasn'" := (tyArr tyStack tyAsn). 
+
+Notation "'tyVarList'" := (tyList tyString).
+Notation "'tyExprList'" := (tyList tyExpr).
+Notation "'tySubstList'" := (tyList (tyPair tyString (tyArr tyStack tyVal))).
 
 Fixpoint type_cast_typ (a b : typ) : option (a = b) :=
   match a as a , b as b return option (a = b) with
@@ -74,6 +84,25 @@ Fixpoint type_cast_typ (a b : typ) : option (a = b) :=
                 end)
         | _ , _ => None
       end
+    | tyPair x y , tyPair a b =>
+      match type_cast_typ x a , type_cast_typ y b with
+        | Some pf , Some pf' =>
+          Some (match pf in _ = t
+                    , pf' in _ = t'
+                      return tyPair x y = tyPair t t'
+                with
+                  | eq_refl , eq_refl => eq_refl
+                end)
+        | _ , _ => None
+      end
+    | tyList x, tyList y =>
+    	match type_cast_typ x y with
+          | Some pf =>
+    		Some (match pf in _ = t return tyList x = tyList t with
+    			    | eq_refl => eq_refl
+    			  end)
+          | None => None
+       end  
     | tyString, tyString => Some eq_refl
     | tyCmd, tyCmd => Some eq_refl
     | tyExpr, tyExpr => Some eq_refl
@@ -81,9 +110,13 @@ Fixpoint type_cast_typ (a b : typ) : option (a = b) :=
     | tyAsn, tyAsn => Some eq_refl
     | tyFields, tyFields => Some eq_refl
     | tySubst, tySubst => Some eq_refl
+
+(*
 	| tyVarList, tyVarList => Some eq_refl
 	| tySubstList, tySubstList => Some eq_refl
 	| tyExprList, tyExprList => Some eq_refl
+*)
+
     | _, _ => None
   end.
   
@@ -94,6 +127,8 @@ Proof.
   split; intros H.
   + destruct a, b; destruct H as [x _]; inversion x; subst; reflexivity.
   + subst. exists eq_refl. induction b; try reflexivity.
+    simpl. rewrite IHb1, IHb2. reflexivity.
+    simpl. rewrite IHb. reflexivity.
     simpl. rewrite IHb1, IHb2. reflexivity.
 Qed.
 
@@ -107,6 +142,8 @@ Lemma type_cast_typ_refl (a : typ) : type_cast_typ a a = Some eq_refl.
 Proof.
   induction a; simpl; try reflexivity.
   rewrite IHa1, IHa2; reflexivity.
+  rewrite IHa. reflexivity.
+  rewrite IHa1, IHa2; reflexivity.
 Qed.
 
 Instance RelDec_correct_typ : RelDec_Correct RelDec_eq_typ.
@@ -117,14 +154,26 @@ Proof.
 	  remember (type_cast_typ x2 y2); destruct o; subst; [|inversion H].
 	  reflexivity.
 	+ do 2 rewrite type_cast_typ_refl; reflexivity.
+	+ remember (type_cast_typ x y); destruct o; subst; [|inversion H].
+	  reflexivity.
+	+ rewrite type_cast_typ_refl. reflexivity.
+	+ remember (type_cast_typ x1 y1); destruct o; subst; [|inversion H].
+	  remember (type_cast_typ x2 y2); destruct o; subst; [|inversion H].
+	  reflexivity.
+	+ do 2 rewrite type_cast_typ_refl; reflexivity.	
 Qed.
 
 Fixpoint typD (ls : list Type) (t : typ) : Type :=
   match t with
     | tyArr a b => typD ls a -> typD ls b
+	| tyList a => @list (typD ls a)
+	| tyPair a b => (typD ls a * typD ls b)%type
+
+(*
     | tyVarList => @list string
     | tyExprList => @list (@Open.expr (String.string) SVal)
     | tySubstList => @list (String.string * (@Open.expr (String.string) SVal))
+*)
     | tyProp => Prop
     | tyNat => nat
     | tySpec => spec
@@ -172,7 +221,7 @@ Instance Typ0_Prop : Typ0 _ Prop :=
 Inductive java_func :=
 | pString (_ : string)
 | pVal (_ : sval)
-| pVarList (_ : @list String.string)
+| pVarList (_ : @list String.string) 
 | pProg (_ : Prog_wf)
 | pCmd (_ : cmd)
 | pExpr (_ : dexpr)
@@ -194,7 +243,7 @@ Inductive java_func :=
 
 | pFieldLookup
 
-| pSetFold
+| pSetFold (_ : typ)
 | pSetFoldFun 
 
 | pStar (_ : typ)
@@ -202,11 +251,17 @@ Inductive java_func :=
 | pLater (_ : typ)
 | pPointsto
 
-| pZipSubst
+| pZip (_ _ : typ)
 | pSubst
 | pTruncSubst
 | pSingleSubst
 
+| pCons (_ : typ)
+| pNil (_ : typ)
+| pLength (_ : typ)
+| pMap (_ _ : typ)
+
+(*
 | pConsVarList
 | pNilVarList
 | pConsExprList
@@ -214,6 +269,7 @@ Inductive java_func :=
 
 | pLengthVarList
 | pLengthExprList
+*)
 
 | pNull.
 
@@ -257,15 +313,24 @@ Definition typeof_sym_java (f : java_func) : option typ :=
     | pFieldLookup => Some (tyArr tyProg (tyArr tyString (tyArr tyFields tyProp)))
     
     | pSetFoldFun => Some (tyArr tyString (tyArr tyString (tyArr tySasn tySasn)))
-    | pSetFold => Some (tyArr (tyArr tyString (tyArr tySasn tySasn)) (tyArr tyFields (tyArr tySasn tySasn)))
+    | pSetFold t => Some (tyArr (tyArr tyString (tyArr t t)) (tyArr tyFields (tyArr t t)))
     
     | pPointsto => Some (tyArr tyVal (tyArr tyString (tyArr tyVal tyAsn)))
     
+    | pZip a b => Some (tyArr (tyList a) (tyArr (tyList b) (tyList (tyPair a b))))
+
+(*
     | pZipSubst => Some (tyArr tyVarList (tyArr tyExprList tySubstList))
+*)
     | pSubst => Some (tyArr tySubstList tySubst)
     | pTruncSubst => Some (tyArr tySubstList tySubst)
     | pSingleSubst => Some (tyArr (tyArr tyStack tyVal) (tyArr tyString tySubst))
     
+    | pCons t => Some (tyArr t (tyArr (tyList t) (tyList t)))
+    | pNil t => Some (tyList t)
+    | pLength t => Some (tyArr (tyList t) tyNat)
+    | pMap a b => Some (tyArr (tyArr a b) (tyArr (tyList a) (tyList b)))
+  (*
     | pConsVarList => Some (tyArr tyString (tyArr tyVarList tyVarList))
     | pNilVarList => Some tyVarList
     | pConsExprList => Some (tyArr (tyArr tyStack tyVal) (tyArr tyExprList tyExprList))
@@ -273,6 +338,7 @@ Definition typeof_sym_java (f : java_func) : option typ :=
     
     | pLengthVarList => Some (tyArr tyVarList tyNat)
     | pLengthExprList => Some (tyArr tyExprList tyNat)
+  *)
     | pNull => Some tyVal
     end.
     
@@ -312,14 +378,23 @@ Definition java_func_eq (a b : java_func) : option bool :=
     | pLater t, pLater u => Some (t ?[ eq ] u)
     | pPointsto, pPointsto => Some true
     | pFieldLookup, pFieldLookup => Some true
-    | pSetFold, pSetFold => Some true
+    | pSetFold t, pSetFold u => Some (t ?[ eq ] u)
     | pSetFoldFun, pSetFoldFun => Some true
+
+	| pZip a b, pZip c d => Some (a ?[ eq ] c && b ?[ eq ] d)%bool
         
+(*
     | pZipSubst, pZipSubst => Some true
+*)
     | pSubst, pSubst => Some true
     | pTruncSubst, pTruncSubst => Some true
     | pSingleSubst, pSingleSubst => Some true
     
+    | pCons t, pCons u => Some (t ?[ eq ] u)
+    | pNil t, pNil u => Some (t ?[ eq ] u)
+    | pLength t, pLength u => Some (t ?[ eq ] u)
+    | pMap a b, pMap c d => Some (a ?[ eq ] c && b ?[ eq ] d)%bool
+(*    
     | pConsVarList, pConsVarList => Some true
     | pNilVarList, pNilVarList => Some true
     | pConsExprList, pConsExprList => Some true
@@ -327,7 +402,7 @@ Definition java_func_eq (a b : java_func) : option bool :=
     
     | pLengthVarList, pLengthVarList => Some true
     | pLengthExprList, pLengthExprList => Some true
-    
+*)   
     | pNull, pNull => Some true
     | _, _ => None
   end.
@@ -347,7 +422,11 @@ Definition set_fold_fun (x : String.string) (f : field) (P : sasn) :=
 	(`pointsto) (x/V) `f `null ** P.
 
 Definition stack_get (x : string) (s : stack) := s x.
-
+Eval cbv in (match typeof_sym_java pSubst with
+  | Some t => typD nil t
+  | None => unit
+  end).
+  Print substlist.
 Instance RSym_imp_func : SymI.RSym java_func :=
 { typeof_sym := typeof_sym_java
 ; symD := fun ts f =>
@@ -391,16 +470,21 @@ Instance RSym_imp_func : SymI.RSym java_func :=
               | pLater _ => tt
               
               | pFieldLookup => field_lookup
-              | pSetFold => @SS.fold (typD ts tySasn)
+              | pSetFold t => @SS.fold (typD ts t)
               | pSetFoldFun => set_fold_fun
               
               | pPointsto => pointsto
               
-              | pZipSubst => zip
+              | pZip a b => @zip (typD ts a) (typD ts b)
               | pSubst => @substl_aux  String.string _ SVal
               | pTruncSubst => @substl_trunc_aux String.string _ SVal
               | pSingleSubst => @subst1 String.string _ SVal
               
+              | pCons t => @cons (typD ts t)
+              | pNil t => @nil (typD ts t)
+              | pLength t => @length (typD ts t)
+              | pMap a b => @map (typD ts a) (typD ts b)
+  (*            
               | pConsVarList => @cons string
               | pNilVarList => @nil string
               | pConsExprList => @cons Open.expr
@@ -408,7 +492,7 @@ Instance RSym_imp_func : SymI.RSym java_func :=
               
               | pLengthVarList => @length string
               | pLengthExprList => @length Open.expr
-              
+  *)            
               | pNull => null
             end
 ; sym_eqb := java_func_eq
@@ -563,11 +647,18 @@ Notation "'fStackGet'" := (Inj (inl (inr pStackGet))).
 Notation "'fStackSet'" := (Inj (inl (inr pStackSet))).
 
 Notation "'fFieldLookup'" := (Inj (inl (inr pFieldLookup))).
-Notation "'fSetFold'" := (Inj (inl (inr pSetFold))).
+Notation "'fSetFold' '[' t ']'" := (Inj (inl (inr (pSetFold t)))).
 Notation "'fSetFoldFun'" := (Inj (inl (inr pSetFoldFun))).
 
+Notation "'fLength' '[' t ']'" := (Inj (inl (inr (pLength t)))).
+Notation "'fNil' '[' t ']'" := (Inj (inl (inr (pNil t)))).
+Notation "'fCons' '[' t ']'" := (Inj (inl (inr (pCons t)))).
+Notation "'fZip' '[' t ',' u ']'" := (Inj (inl (inr (pZip t u)))).
+Notation "'fMap' '[' t ',' u ']'" := (Inj (inl (inr (pMap t u)))).
+(*
 Notation "'fLengthVarList'" := (Inj (inl (inr pLengthVarList))).
 Notation "'fLengthExprList'" := (Inj (inl (inr pLengthExprList))).
+*)
 
 Notation "'fTypeOf'" := (Inj (inl (inr pTypeOf))).
 
@@ -584,14 +675,19 @@ Notation "'mkMethodSpec' '[' C ',' m ',' args ',' r ',' p ',' q ']'" :=
     (App (App (App (App (App (App fMethodSpec C) m) args) r) p) q) (at level 0).
 Notation "'mkTriple' '[' P ',' c ',' Q ']'" := (App (App (App fTriple P) Q) c) (at level 0).
 Notation "'mkFieldLookup' '[' P ',' C ',' f ']'" := (App (App (App fFieldLookup P) C) f) (at level 0).
-Notation "'mkSetFold' '[' x ',' f ',' P ']'" := (App (App (App fSetFold (App fSetFoldFun x)) f) P). 
+Notation "'mkSetFold' '[' t ',' x ',' f ',' P ']'" := (App (App (App (fSetFold [t]) (App fSetFoldFun x)) f) P). 
 Notation "'mkTypeOf' '[' C ',' x ']'" := (App (App fTypeOf C) x) (at level 0).
 
+Notation "'mkCons' '[' t ',' x ',' xs ']'" := (App (App (fCons [t]) x) xs).
+Notation "'mkLength '[' t ',' lst ']'" := (App (fLength [t]) lst).
+
+(*
 Notation "'mkNilVarList'" := (Inj (inl (inr pNilVarList))) (at level 0).
 Notation "'mkNilExprList'" := (Inj (inl (inr pNilExprList))) (at level 0).
 Notation "'mkConsVarList' '[' x ',' xs ']'" := (App (App (Inj (inl (inr pConsVarList))) x) xs) (at level 0).
 Notation "'mkConsExprList' '[' x ',' xs ']'" := (App (App (Inj (inl (inr pConsExprList))) x) xs) (at level 0).
-	
+*)
+
 Notation "'mkVal' '[' v ']'" := (Inj (inl (inr (pVal v)))) (at level 0).
 Notation "'mkVarList' '[' lst ']'" := (Inj (inl (inr (pVarList lst)))) (at level 0).
 
@@ -601,14 +697,23 @@ Notation "'mkProgEq' '[' P ']'" := (App fProgEq P) (at level 0).
 Notation "'mkCmd' '[' c ']'" := (Inj (inl (inr (pCmd c)))) (at level 0).
 Notation "'mkExpr' '[' e ']'" := (Inj (inl (inr (pExpr e)))) (at level 0).
 Notation "'mkFields' '[' fs ']'" := (Inj (inl (inr (pFields fs)))) (at level 0).
+Check fold_right.
 
-Notation "'mkExprList' '[' lst ']'" := (fold_right (fun e acc => mkConsExprList [App fEval (mkExpr [e]), acc]) mkNilExprList lst) (at level 0).
+Notation "'mkExprList' '[' es ']'" :=
+	(fold_right (fun (e : dexpr) (acc : expr typ func) => 
+		mkCons [tyExpr, mkExpr [e], acc]) (fNil [tyExpr]) es).
+
+(*
+Notation "'mkExprList' '[' lst ']'" := (fold_right (fun e acc => mkCons [tyExpr, App fEval (mkExpr [e]), acc]) (mkNil [tyExpr]) lst) (at level 0).
+*)
 
 Notation "'mkConst' '[' t ',' a ']'" := (App (fConst [t]) a) (at level 0).
 Notation "'mkEval' '[' e ',' s ']'" := (App (App fEval e) s) (at level 0).
 
+(*
 Notation "'mkLengthVarList' '[' lst ']'" := (App fLengthVarList lst).
 Notation "'mkLengthExprList' '[' lst ']'" := (App fLengthExprList lst).
+*)
 
 Notation "'mkEq' '[' t ',' a ',' b ']'" := (App (App (fEq [t]) a) b).
 
@@ -618,6 +723,8 @@ Notation "'fAnd' '[' l ']'" := (Inj (inr (ilf_and l))).
 Notation "'fOr' '[' l ']'" := (Inj (inr (ilf_or l))).
 Notation "'fImpl' '[' l ']'" := (Inj (inr (ilf_impl l))).
 Notation "'fEntails' '[' l ']'" := (Inj (inr (ilf_entails l))).
+
+Notation "'fLater' '[' l ']'" := (Inj (inl (inr (pLater l)))).
 
 Notation "'mkExists' '[' l ',' t ',' e ']'" := (App (fExists [l, t]) (Abs t e)).
 Notation "'mkForall' '[' l ',' t ',' e ']'" := (App (fForall [l, t]) (Abs t e)).
@@ -647,10 +754,12 @@ Notation "'mkApplySubst' '[' t ',' P ',' es ']'" := (mkApplySubst [t, P, mkSubst
 
 Notation "'mkTruncSubst' '[' es ']'" := (App fTruncSubst es).
 Notation "'mkApplyTruncSubst' '[' t ',' P ',' es ']'" := (mkApplySubst [t, P, mkTruncSubst [es]]).
-                                                         
+ 
+(*                                                        
 Notation "'mkSubstList' '[' vs ',' es ']'" := (App (App (Inj (inl (inr pZipSubst))) vs) es) (at level 0).
 
 Notation "'mkSubstExprList' '[' lst ',' x ',' v ']'" := (fold_right (fun e acc => mkConsExprList [mkApplySingleSubst[tyVal, App fEval (mkExpr [e]), x, v], acc]) mkNilExprList lst).
+*)
 
 Notation "'mkNull'" := (Inj (inl (inr pnull))).
 
